Case_Study/RT_Log.thy
@@ -4,7 +4,7 @@ imports RT_Map
 
 begin
 
-
+(*
 consts root_log_low :: "paddr"
 
 consts root_log_high :: "paddr"
@@ -14,30 +14,41 @@ definition
   "root_log_fp = map Addr [addr_val root_log_low .e. addr_val root_log_high]"
 
 definition
-  root_log :: "p_state \<Rightarrow> paddr list"
+  root_log' :: "p_state \<Rightarrow> paddr list"
 where
-  "root_log s  =  map (Addr o the o heap s) root_log_fp"
+  "root_log' s  =  map (Addr o the o heap s) root_log_fp"
+*)
+
+
+definition
+  root_log :: "p_state \<Rightarrow> paddr set"
+where
+  "root_log s  = {r. \<exists>a. root_map s r = Some a}"
+
 
 
 
 lemma [simp]:
   "root_log s = root_log (s \<lparr>incon_set := is\<rparr>)"
-  by (clarsimp simp: root_log_def)
+  by (clarsimp simp: root_log_def root_map_def map_of_set_def  root_set_def)
 
 lemma [simp]:
   "root_log (s \<lparr>heap := h , incon_set := is\<rparr>) = root_log (s \<lparr>heap := h\<rparr>)"
-  by (clarsimp simp: root_log_def)
+  by (clarsimp simp: root_log_def root_map_def map_of_set_def  root_set_def)
 
+(*
 lemma  rootI:
   "p \<notin> set root_log_fp \<Longrightarrow> root_log (s \<lparr>heap := heap s (p \<mapsto> v1)\<rparr>) = root_log s"
-  by (clarsimp simp: root_log_def)
+  by (clarsimp simp: root_log_def root_map_def map_of_set_def  root_set_def)
 
 
 lemma  rootI1:
   "\<lbrakk>p \<notin> set root_log_fp; p1 \<notin> set root_log_fp \<rbrakk> \<Longrightarrow> 
     root_log (s \<lparr>heap := heap s (p \<mapsto> v1 , p1 \<mapsto> v2)\<rparr>) = root_log s"
   by (auto simp: root_log_def)
- 
+
+*)
+
 (* assumption of non-sharing address space of the processes, pages can be shared, but even 
    then every process will have its own  page table entry *)
 
@@ -46,14 +57,17 @@ definition
   non_overlapping_defined_page_tables :: "p_state \<Rightarrow> bool"
 where
   "non_overlapping_defined_page_tables s \<equiv> 
-                     \<forall>x y. x\<in> set (root_log s) \<and> y \<in> set (root_log s) \<and>
+                     \<forall>x y. x\<in>(root_log s) \<and> y \<in> (root_log s) \<and>
                               x\<noteq>y \<longrightarrow> \<Union>(ptable_trace' (heap s) x ` UNIV) \<inter> \<Union>(ptable_trace' (heap s) y ` UNIV) = {}"
 
+lemma 
+  "root_map s r = Some a  \<longrightarrow> r \<in> root_log s"
+  by (clarsimp simp: root_log_def)
 
 
 definition
   "asids_consistent S s \<equiv>  
-           (\<forall> r a. root_map s r = Some a  \<and> r \<in> set (root_log s) \<longrightarrow> a \<notin> S \<union> {asid s}  \<longrightarrow> 
+           (\<forall> r a. root_map s r = Some a  \<longrightarrow> a \<notin> S \<union> {asid s}  \<longrightarrow> 
                   (\<forall>v. (ptable_snapshot s) a v \<noteq> Incon \<and> ((ptable_snapshot s) a v = Miss \<or> 
                                  (ptable_snapshot s) a v = Hit (pt_walk a (heap s) r v) )))"
 
